update

PVS_Assignment/ex_09_Hoangkim/ex_09_Hoangkim.dfy
@@ -1,5 +1,66 @@
-method rotateLeft<T>(a:array<T>)
-modifies a
+//problem 01
+//problem 02
+
+method rotateLeft<T>(a: array<T>)
+  modifies a
+  requires a.Length > 0
 {
-    
+  var len := a.Length;
+  var i := 0;
+
+  while (i < len)
+    invariant 0 <= i <= len
+    invariant  multiset(a[..]) == multiset(old(a[..]))
+  {
+    var temp := a[(i + 1) % len];
+    a[(i + 1) % len] := a[i];
+    a[i] := temp;
+    i := i + 1;
+  }
 }
+
+
+//Problem03
+// Ghost predicate to represent a sorted sequence
+ghost predicate sorted(a:seq<int>)
+{∀ i,j | 0 ≤  i < j  < |a| :: a[i] ≤ a[j] }
+
+method InsertionSort(a:array<int>)
+  modifies a
+  requires a.Length ≥ 2
+  ensures sorted(a[..])
+  ensures multiset(a[..]) == multiset(old(a[..]))
+{
+  var x := 1;
+  while x < a.Length
+    invariant 1 ≤ x ≤ a.Length;
+    invariant sorted(a[..x]);
+    invariant multiset(a[..]) == multiset(old(a[..]))
+  {
+
+
+    var i := x;
+    var d := x;
+
+    x := x + 1;
+
+    var temp := a[i];  // Save the value of the element to be inserted
+
+    while d >= 1 && a[d - 1] > temp
+      invariant 0 ≤ d ≤ i + 1;
+      invariant forall i, j | 0 ≤ i < j < d :: a[i] ≤ a[j];  // Elements before position d are sorted
+    {
+      a[d] := a[d - 1];  // Copy the next element into place
+      d := d - 1;
+    }
+    a[d] := temp;  // Write the saved value into place
+  
+  }
+}
+
+
+
+
+
+
+
